Simplify subparser behavior

AllStar/Subparser.v
@@ -1,117 +1,108 @@
 Require Import Bool List String.
-
 Require Import Grammar Lib.Utils.
 Import ListNotations.
 Open Scope string_scope.
 
 Record subparser :=
-  mkSp { busy       : list symbol ; (* use a set instead? *)
-         syms       : list symbol ;
-         input      : list string ;
-         prediction : list symbol ;
-         stack      : list (list symbol) }.
+  mkSp { stack      : list symbol ;
+         prediction : list symbol }.
 
-Definition rhss (g : grammar) (x : string) :=
-  map snd (filter (fun prod => beqSym (fst prod) (NT x)) g).
+Definition beqSp sp sp2 :=
+  beqList sp.(stack) sp2.(stack) &&
+  beqList sp.(prediction) sp2.(prediction).
 
-Definition moveSubparser (g  : grammar)
-                         (sp : subparser) :
-                         list subparser :=
-  let (busy, syms, input, prediction, stack) := sp in
-  match syms with
-  | nil =>
-    match (stack, busy) with
-    | (nil, nil) => [sp]
-    | (k :: stack', b :: busy') => [mkSp busy' k input prediction stack']
-    | _ => [mkSp nil nil ["implementation error"] nil nil]
-    end
-  | T y :: syms' =>
-    match input with
-    | nil => nil
-    | token :: input' =>
-      match beqSym (T y) (T token) with
-      | false => nil
-      | true => [mkSp nil syms' input' prediction stack]
+Definition moveSp (g : grammar)
+    (token : string) (sp : subparser) : list subparser :=
+  match sp.(stack) with
+  | nil => nil
+  | NT _ :: _ => [sp]
+  | T y :: stack' =>
+    if beqSym (T y) (T token) then
+      [mkSp stack' sp.(prediction)]
+    else
+      nil
+  end.
+
+Definition move (g : grammar) (sps : list subparser) (token : string) : list subparser :=
+  concat (map (moveSp g token) sps).
+
+Fixpoint spClosure (g    : grammar)
+                   (busy : list subparser)
+                   (fuel : nat)
+                   (sp   : subparser)
+                   : list subparser :=
+  match fuel with
+  | O => nil
+  | S n => 
+    if elem sp busy beqSp then
+      nil
+    else
+      match sp.(stack) with
+      | nil => [sp]
+      | T _ :: _ => [sp]
+      | NT x :: stack' =>
+        let gammas := rhss g x in
+        let newSps :=
+            map (fun gamma =>
+                   mkSp (gamma ++ stack') sp.(prediction))
+                gammas
+        in concat (map (spClosure g (sp :: busy) n) newSps)
       end
-    end
-  | NT x :: k =>
-    match find (beqSym (NT x)) busy with
-    | Some _ => nil (* changed from [sp] *)
-    | None =>
-      let mkSp' := fun gamma => mkSp (NT x :: busy) 
-                                     gamma 
-                                     input 
-                                     prediction 
-                                     (k :: stack) in
-      let xGammas := rhss g x in
-      map mkSp' xGammas
-    end
   end.
 
-Definition startState g x input :=
-  let xGammas := rhss g x in
-  map (fun gamma =>
-         mkSp [NT x] gamma input gamma [[]]) xGammas.
+Definition closure (g : grammar) (sps : list subparser) :=
+  concat (map (spClosure g nil 100) sps).
 
-Definition target g sps :=
-  concat (map (moveSubparser g) sps).
+Definition startState g x stack0 :=
+  let gammas := rhss g x in
+  let sps    := map (fun gamma =>
+                       mkSp (gamma ++ stack0) gamma) gammas
+  in  closure g sps.
 
-Definition elem {A : Type} (x : A) (l : list A) (cmp : A -> A -> bool) : bool :=
-            match find (cmp x) l with
-  | Some _ => true
-  | None   => false
-  end.
-
-Definition nub {A : Type} (xs : list A) (cmp : A -> A -> bool) : list A :=
-  fold_right (fun x acc => if elem x acc cmp then acc else x :: acc) nil xs.
-
-Fixpoint beqList (xs : list symbol) (ys : list symbol) : bool :=
-  match (xs, ys) with
-  | (nil, nil) => true
-  | (x :: xs', y :: ys') => if beqSym x y then beqList xs' ys' else false
-  | _ => false
-  end.
-
-Fixpoint beqStack (xss yss : list (list symbol)) : bool :=
-  match (xss, yss) with
-  | (nil, nil) => true
-  | (xs :: xss', ys :: yss') => if beqList xs ys then beqStack xss' yss' else false
-  | _ => false
-  end.
+Definition target g sps (token : string) :=
+  closure g (move g sps token ).
 
 Fixpoint conflict sps : bool :=
   match sps with
   | nil => false
-  | [sp] => false
   | sp :: sps' => 
-    if existsb (fun sp2 => 
-                  beqList sp.(syms) sp2.(syms) && 
-                  beqStack sp.(stack) sp2.(stack) &&
-                  negb (beqList sp.(prediction) sp2.(prediction))) sps'
+    if existsb
+         (fun sp2 => 
+            beqList sp.(stack) sp2.(stack) && 
+            negb (beqList sp.(prediction)                                                sp2.(prediction)))
+         sps'
     then true
     else conflict sps'
   end.
 
-Inductive sll_result := 
-| Choice   : list symbol -> sll_result
-| Conflict : list subparser -> sll_result
-| Fail     : sll_result.  
+Inductive prediction_result := 
+| Choice   : list symbol -> prediction_result
+| Conflict : list subparser -> prediction_result
+| Fail     : prediction_result.  
 
-Fixpoint sllPredict g sps fuel :=
-  match fuel with
-  | O => Fail
-  | S n =>
-    let predictions := map prediction sps in
-    match nub predictions beqList with
-    | nil => Fail
-    | [p] => Choice p
-    | _ => if conflict sps then
-             Conflict sps
-           else 
-             sllPredict g (target g sps) n
-    end
+(* LL predict when initial stacks are nil,
+   SLL predict otherwise *)
+Fixpoint predict g sps input :=
+  let predictions := map prediction sps in
+  match nub predictions beqList with
+  | nil => Fail
+  | [p] => Choice p
+  | _ => if conflict sps then
+           Conflict sps
+         else
+           match input with
+           | nil => Fail (*actually, check for final configs*)
+           | token :: input' => 
+             predict g (target g sps token) input'
+           end
   end.
 
-Definition adaptivePredict g x input :=
-  sllPredict g (startState g x input) 100.
-             
+Definition adaptivePredict g x input stack0 :=
+  let sllPrediction :=
+      predict g (startState g x nil) input
+  in  match sllPrediction with
+      | Conflict _ =>
+        predict g (startState g x stack0) input
+      | _ => sllPrediction
+      end.
+
